# See details within this document for linkage to specification and purpose.
# This ontology file is a non-normative supporting document.
@prefix rdfs: <http://www.w3.org/2000/01/rdf-schema#>.
@prefix owl: <http://www.w3.org/2002/07/owl#>.
@prefix rdf: <http://www.w3.org/1999/02/22-rdf-syntax-ns#>.
@prefix dcterms: <http://purl.org/dc/terms/>.
@prefix vs: <http://www.w3.org/2003/06/sw-vocab-status/ns#> .
@prefix : <http://www.w3.org/ns/ldp#>.

:
	a owl:Ontology;
    dcterms:description "Vocabulary URIs defined in the Linked Data Platform Paging (LDP-Paging) namespace.";
	dcterms:title "The W3C Linked Data Platform Paging (LDP-Paging) Vocabulary";
	rdfs:label "W3C Linked Data Platform Paging (LDP-Paging)";
	rdfs:comment "This ontology provides an informal representation of the concepts and terms
	as defined in the LDP specification.  Consult the LDP specification for normative reference.";
	rdfs:seeAlso <http://www.w3.org/2012/ldp>,
		<http://www.w3.org/TR/ldp-ucr/>,
		<http://www.w3.org/TR/ldp/>,
		<http://www.w3.org/TR/ldp-paging/>,
		<http://www.w3.org/2011/09/LinkedData/>.
			
:containerSortCriteria
 	a rdf:Property;
	rdfs:comment "Link to the list of sorting criteria used by the server in a representation.";
	vs:term_status "unstable";
	rdfs:domain :Page;
	rdfs:isDefinedBy :;
	rdfs:label "containerSortCriteria";
	rdfs:range rdf:List.
	
:ContainerSortCriterion
 	a rdf:Class;
	rdfs:comment "Element in the list of container sorting criteria used by the server in a representation.";
	vs:term_status "unstable";
	rdfs:label "ContainerSortCriterion";
	rdfs:isDefinedBy :.
	
:containerSortPredicate
 	a rdf:Property;
	rdfs:comment "Predicate used to determine the order of the members in a page.";
	vs:term_status "unstable";
	rdfs:domain :ContainerSortCriterion;
	rdfs:isDefinedBy :;
	rdfs:label "containerSortPredicate";
	rdfs:range rdf:Property.
	
:containerSortOrder
 	a rdf:Property;
	rdfs:comment "The ascending/descending/etc order used to order the members in a page.";
	vs:term_status "unstable";
	rdfs:domain :ContainerSortCriterion;
	rdfs:isDefinedBy :;
	rdfs:label "containerSortOrder";
	rdfs:range rdf:Resource.
	
:containerSortCollation
 	a rdf:Property;
	rdfs:comment "The collation used to order the members in a page when comparing strings.";
	vs:term_status "unstable";
	rdfs:domain :ContainerSortCriterion;
	rdfs:isDefinedBy :;
	rdfs:label "containerSortCollation";
	rdfs:range rdf:Property.
	
:Ascending
 	a rdf:Description;		# individual
	rdfs:comment "Ascending order.";
	vs:term_status "unstable";
	rdfs:isDefinedBy :;
	rdfs:label "Ascending".
	
:Descending
 	a rdf:Description;		# individual
	rdfs:comment "Descending order.";
	vs:term_status "unstable";
	rdfs:isDefinedBy :;
	rdfs:label "Descending".
	
:Page
	a rdfs:Class;
	rdfs:comment "A resource that represents a limited set of members of a LDP Container.";
	vs:term_status "unstable";
	rdfs:isDefinedBy :;
	rdfs:label "Page".