
<rdf:RDF xmlns="http://www.w3.org/2004/08/Presentations.owl#"
		xmlns:rdf="http://www.w3.org/1999/02/22-rdf-syntax-ns#"
		xmlns:rdfs="http://www.w3.org/2000/01/rdf-schema#"
		xmlns:owl="http://www.w3.org/2002/07/owl#"
		xmlns:ical="http://www.w3.org/2002/12/cal/ical#"
		xmlns:org="http://www.w3.org/2001/04/roadmap/org#"
		xmlns:contact="http://www.w3.org/2000/10/swap/pim/contact#"
		xmlns:dc="http://purl.org/dc/elements/1.1/"
		xmlns:vcard="http://www.w3.org/2001/vcard-rdf/3.0#">
	<owl:Ontology rdf:about="">
		<rdfs:label>Ontology used to manage presentations at W3C</rdfs:label>
		<dc:creator>Ivan Herman</dc:creator>
		<owl:versionInfo>$Id: Presentations.owl,v 1.7 2006/05/05 09:12:16 ivan Exp $</owl:versionInfo>
		<dc:publisher>World Wide Web Consortium</dc:publisher>
		<rdfs:comment>
		2005-02-01: based on DanC's comment, I changed the usage of org:name to 
		include a separate resource that can be used as a subject for this property. (The previous
		usage misused org:name)
		2005-05-02: added a dc:coverage property for a talk, used to indicate the end of an event if needed (currently used
		for booth-s that are ran at an event)
		</rdfs:comment>
	</owl:Ontology>	
	<!-- ==================================================================================================== -->
	<owl:Class rdf:ID="Talk">
		<rdfs:comment>Date of the presentation</rdfs:comment>
		<rdfs:subClassOf>
			<owl:Restriction>
				<owl:onProperty rdf:resource="http://purl.org/dc/elements/1.1/date"/>
				<owl:cardinality rdf:datatype="http://www.w3.org/2001/XMLSchema#integer">1</owl:cardinality>
			</owl:Restriction>
		</rdfs:subClassOf>
		<rdfs:comment>This is used for the end date of an event (eg, for booth-s)</rdfs:comment>
		<rdfs:subClassOf>
			<owl:Restriction>
				<owl:onProperty rdf:resource="http://purl.org/dc/elements/1.1/coverage"/>
				<owl:maxCardinality rdf:datatype="http://www.w3.org/2001/XMLSchema#integer">1</owl:maxCardinality>
			</owl:Restriction>
		</rdfs:subClassOf>
		
		<rdfs:comment>A talk may have one or several presentors. In the latter case, the order of the presentors might be important, 
		     hence the separation of the two cases (and that is the reason I did not want to use dc:creator)</rdfs:comment>
		<rdfs:subClassOf>
			<owl:Class>
				<owl:unionOf rdf:parseType="Collection">
					<owl:Class rdf:about="#OnePresenterTalk"/>
					<owl:Class rdf:about="#MultiplePresenterTalk"/>
				</owl:unionOf>
			</owl:Class>
		</rdfs:subClassOf>
		
		<rdfs:comment>Title of the presentation, possibly in the original language. One would expect the cardinality to be exactly 
		    one, but I found talks in the list that have no title (I am not sure we should accept those, b.t.w....)</rdfs:comment>
		<rdfs:subClassOf>
			<owl:Restriction>
				<owl:onProperty rdf:resource="http://purl.org/dc/elements/1.1/title"/>
				<owl:maxCardinality rdf:datatype="http://www.w3.org/2001/XMLSchema#integer">1</owl:maxCardinality>
			</owl:Restriction>
		</rdfs:subClassOf>
		<rdf:comment>This restriction is, in fact, only to emphasize the usage of the language term of DC. We can 'agree' that 
			if there is no language property used, than the language is US English. Otherwise it should be set</rdf:comment>
		<rdfs:subClassOf>
			<owl:Restriction>
				<owl:onProperty rdf:resource="http://purl.org/dc/elements/1.1/language"/>
				<owl:maxCardinality rdf:datatype="http://www.w3.org/2001/XMLSchema#integer">1</owl:maxCardinality>
			</owl:Restriction>
		</rdfs:subClassOf>
		<rdfs:comment>Title of the presentation translated to English (in case the title is not in English). It is a pity, b.t.w., 
		   that no such distinction exists in the Dublin Core. Oh well...
           This is, admittingly, a bit awkward. What I would like here to have is to say: 'if the language tag is set, then the 
		   cardinality of dc:title is '2', one of the dc:title must be in English, the other in the language set by 'dc:language'. 
		   This is not expressable in OWL, I am not sure about SWRL or cwm either, but I would hope so. For the time being, I 
		   therefore chose to separate the two into different properties.</rdfs:comment>
		<rdfs:subClassOf>
			<owl:Restriction>
				<owl:onProperty rdf:resource="#translatedTitle"/>
				<owl:maxCardinality rdf:datatype="http://www.w3.org/2001/XMLSchema#integer">1</owl:maxCardinality>
			</owl:Restriction>
		</rdfs:subClassOf>
		
		<rdfs:comment>Identify W3C Office organizing the event (if applicable, ie, the minimum cardinality is 0)</rdfs:comment>
		<rdfs:subClassOf>
			<owl:Restriction>
				<owl:onProperty rdf:resource="#office"/>
				<owl:maxCardinality rdf:datatype="http://www.w3.org/2001/XMLSchema#integer">1</owl:maxCardinality>
			</owl:Restriction>
		</rdfs:subClassOf>
		
		<rdfs:comment>Identify the activity, domain,etc relevant for the presentation. The object resource 
		    should be such that the http://www.w3.org/2001/04/roadmap/org#name can be used on it to identify a W3C
		    activity, group, etc.</rdfs:comment>
		<rdfs:subClassOf>
			<owl:Restriction>
				<owl:onProperty rdf:resource="#w3cActivity"/>
				<owl:minCardinality rdf:datatype="http://www.w3.org/2001/XMLSchema#integer">0</owl:minCardinality>
			</owl:Restriction>
		</rdfs:subClassOf>
		
		<rdfs:subClassOf>
			<owl:Restriction>
				<owl:onProperty rdf:resource="http://www.w3.org/2001/04/roadmap/org#name"/>
				<owl:minCardinality rdf:datatype="http://www.w3.org/2001/XMLSchema#integer">0</owl:minCardinality>
			</owl:Restriction>
		</rdfs:subClassOf>
		<rdfs:comment>Identify the type of talk (typically: tutorial, invited talk, etc)</rdfs:comment>
		<rdfs:subClassOf>
			<owl:Restriction>
				<owl:onProperty rdf:resource="#type"/>
				<owl:minCardinality rdf:datatype="http://www.w3.org/2001/XMLSchema#integer">0</owl:minCardinality>
			</owl:Restriction>
		</rdfs:subClassOf>
		<rdfs:comment>URI of slides. In earlier versions there was a separate property here, but I realized
		    that the dc:identifier is perfectly o.k. here!</rdfs:comment>
		<rdfs:subClassOf>
			<owl:Restriction>
				<owl:onProperty rdf:resource="http://purl.org/dc/elements/1.1/identifier"/>
				<owl:maxCardinality rdf:datatype="http://www.w3.org/2001/XMLSchema#integer">1</owl:maxCardinality>
			</owl:Restriction>
		</rdfs:subClassOf>
		<rdfs:comment>Event where the presentation takes place</rdfs:comment>
		<rdfs:subClassOf>
			<owl:Restriction>
				<owl:onProperty rdf:resource="#event"/>
				<owl:maxCardinality rdf:datatype="http://www.w3.org/2001/XMLSchema#integer">1</owl:maxCardinality>
			</owl:Restriction>
		</rdfs:subClassOf>
	</owl:Class>
	
	<!-- ================================================================================ -->
	<owl:DeprecatedProperty rdf:ID="organization">
		<rdfs:label>Identify 'organizational unit on behalf of which the presentation is made.</rdfs:label>
		<rdfs:comment>The 'organizational unit' might be a WG or an activity, for example. At present, only
		a string is required, at some point one might want to list allowable alternatives here...</rdfs:comment>
		<rdfs:comment>The property below took its place... (this was defined as a datatype property, 
		that was wrong...)</rdfs:comment>
	</owl:DeprecatedProperty>
	
	<owl:ObjectProperty rdf:ID="w3cActivity">
		<rdfs:label>Identify 'organizational unit on behalf of which the presentation is made.</rdfs:label>
		<rdf:comment>The current scripts rely on an org:name to identify an activity</rdf:comment>
		<rdfs:domain rdf:resource="#Talk"/>
		<rdfs:range rdf:resource="http://www.w3.org/2001/04/roadmap/org#Activity"/>
	</owl:ObjectProperty>
	
	<owl:DatatypeProperty rdf:ID="office">
		<rdfs:label>Identify 'organizational unit on behalf of which the presentation is made.</rdfs:label>
		<rdfs:comment>At present, only a string is required, at some point one might want to list allowable alternatives here...</rdfs:comment>
		<rdfs:domain rdf:resource="#Talk"/>
		<rdfs:range rdf:resource="http://www.w3.org/2001/XMLSchema#string"/>
	</owl:DatatypeProperty>
	
	<owl:ObjectProperty rdf:ID="event">
		<rdfs:label>The event where the presentation takes place</rdfs:label>
		<rdfs:domain rdf:resource="#Talk"/>
		<rdfs:range rdf:resource="#Event"/>
	</owl:ObjectProperty>
	
	<owl:DatatypeProperty rdf:ID="translatedTitle">
		<rdfs:label>Title in English</rdfs:label>
		<rdfs:domain rdf:resource="#Talk"/>
		<rdfs:range rdf:resource="http://www.w3.org/2001/XMLSchema#string"/>
	</owl:DatatypeProperty>
	
	<!-- It is really a pain that one cannot use the parseType="Collection" here... -->
	<owl:DatatypeProperty rdf:ID="type">
		<rdfs:label>Type of talk</rdfs:label>
		<rdfs:comment>At some point a better classification of talk type might become necessary. For the time being, this reflects the usage of the system, and
		we will see what comes up in practice.</rdfs:comment>
		<rdfs:domain rdf:resource="#Talk"/>
		<rdfs:range>
			<owl:DataRange>
				<rdf:oneOf>
					<rdf:List>
						<rdf:first rdf:datatype="http://www.w3.org/2001/XMLSchema#string">talk</rdf:first>
						<rdf:rest>
							<rdf:List>
								<rdf:first rdf:datatype="http://www.w3.org/2001/XMLSchema#string">invited talk</rdf:first>
								<rdf:rest>
									<rdf:List>
										<rdf:first rdf:datatype="http://www.w3.org/2001/XMLSchema#string">keynote</rdf:first>
										<rdf:rest>
											<rdf:List>
												<rdf:first rdf:datatype="http://www.w3.org/2001/XMLSchema#string">tutorial</rdf:first>
												<rdf:rest>
													<rdf:List>
														<rdf:first rdf:datatype="http://www.w3.org/2001/XMLSchema#string">state of the art report</rdf:first>
														<rdf:rest>
															<rdf:List>
																<rdf:first rdf:datatype="http://www.w3.org/2001/XMLSchema#string">lecture</rdf:first>
																<rdf:rest>
																	<rdf:List>
																		<rdf:first rdf:datatype="http://www.w3.org/2001/XMLSchema#string">panel</rdf:first>
																		<rdf:rest>
																			<rdf:List>
																				<rdf:first rdf:datatype="http://www.w3.org/2001/XMLSchema#string">lunchtime talk</rdf:first>
																				<rdf:rest>
																					<rdf:List>
																						<rdf:first rdf:datatype="http://www.w3.org/2001/XMLSchema#string">run(s) a booth</rdf:first>
																						<rdf:rest rdf:resource="http://www.w3.org/1999/02/22-rdf-syntax-ns#nil"/>
																					</rdf:List>
																				</rdf:rest>
																			</rdf:List>
																		</rdf:rest>
																	</rdf:List>
																</rdf:rest>
															</rdf:List>
														</rdf:rest>
													</rdf:List>
												</rdf:rest>
											</rdf:List>
										</rdf:rest>
									</rdf:List>
								</rdf:rest>
							</rdf:List>
						</rdf:rest>
					</rdf:List>
				</rdf:oneOf>
			</owl:DataRange>
		</rdfs:range>
	</owl:DatatypeProperty>
	
	
	<!-- ============================================================================================== -->
	
	<owl:Class rdf:nodeID="OnePresenterTalk">
		<rdfs:comment>The name of the Class tells it all...</rdfs:comment>
		<owl:disjointWith rdf:resource="#MultiplePresenterTalk"/>
		<rdfs:comment>There must be exactly one presenter</rdfs:comment>
		<rdfs:subClassOf>
			<owl:Restriction>
				<owl:onProperty rdf:resource="#presenter"/>
				<owl:cardinality rdf:datatype="http://www.w3.org/2001/XMLSchema#nonNegativeInteger">1</owl:cardinality>
			</owl:Restriction>
		</rdfs:subClassOf>
		<rdfs:comment>There must be *no* presenters(!)</rdfs:comment>
		<rdfs:subClassOf>
			<owl:Restriction>
				<rdfs:comment>The case when there are more presenters</rdfs:comment>
				<owl:onProperty rdf:resource="#presenters"/>
				<owl:cardinality rdf:datatype="http://www.w3.org/2001/XMLSchema#integer">0</owl:cardinality>
			</owl:Restriction>
		</rdfs:subClassOf>
	</owl:Class>
	<owl:Class rdf:nodeID="MultiplePresenterTalk">
		<rdfs:comment>The name of the Class tells it all...</rdfs:comment>
		<rdfs:comment>There must be *no* presenter(!)</rdfs:comment>
		<rdfs:subClassOf>
			<owl:Restriction>
				<owl:onProperty rdf:resource="#presenter"/>
				<owl:cardinality rdf:datatype="http://www.w3.org/2001/XMLSchema#nonNegativeInteger">0</owl:cardinality>
			</owl:Restriction>
		</rdfs:subClassOf>
		<rdfs:comment>There must be exactly one presenters(!)</rdfs:comment>
		<rdfs:subClassOf>
			<owl:Restriction>
				<rdfs:comment>The case when there are more presenters</rdfs:comment>
				<owl:onProperty rdf:resource="#presenters"/>
				<owl:cardinality rdf:datatype="http://www.w3.org/2001/XMLSchema#integer">1</owl:cardinality>
			</owl:Restriction>
		</rdfs:subClassOf>
	</owl:Class>
	<owl:Class rdf:nodeID="ListOfPersons">
		<rdfs:label>A list whose constituents *must* be persons</rdfs:label>
		<rdfs:comment>Note that this Class specification, and the typing of rdf:nil below,
		    make this OWL be non-DL (There must be no restriction imposed on rdfs properties in DL...)</rdfs:comment>
		<rdfs:subClassOf rdf:resource="http://www.w3.org/1999/02/22-rdf-syntax-ns#List"/>
		<rdfs:subClassOf>
			<owl:Restriction>
				<!-- all the elements of the list are Persons -->
				<owl:onProperty rdf:resource="http://www.w3.org/1999/02/22-rdf-syntax-ns#first"/>
				<owl:allValuesFrom rdf:resource="http://www.w3.org/2000/10/swap/pim/contact#Person"/>
			</owl:Restriction>
		</rdfs:subClassOf>
		<rdfs:subClassOf>
			<owl:Restriction>
				<!-- all the sublists are also of the same type, or possibly nil -->
				<owl:onProperty rdf:resource="http://www.w3.org/1999/02/22-rdf-syntax-ns#rest"/>
				<owl:allValuesFrom rdf:resource="#ListOfPersons"/>
			</owl:Restriction>
		</rdfs:subClassOf>
	</owl:Class>
	<rdf:Description rdf:about="http://www.w3.org/1999/02/22-rdf-syntax-ns#nil">
		<rdf:comment>This type setting is necessary to close the lists and fufill the restriction on
		    rdf:rest set in ListOfPersons...
			This definitely kicks the ontology out of OWL DL, though...</rdf:comment>
		<rdf:type rdf:resource="http://www.w3.org/1999/02/22-rdf-syntax-ns#List"/>
	</rdf:Description>
	<owl:ObjectProperty rdf:ID="presenter">
		<rdfs:label>Presentor</rdfs:label>
		<rdfs:comment>A single presenter may refer to one person only</rdfs:comment>
		<rdfs:domain rdf:resource="#OnePresenterTalk"/>
		<rdfs:range rdf:resource="http://www.w3.org/2000/10/swap/pim/contact#Person"/>
	</owl:ObjectProperty>
	<owl:ObjectProperty rdf:ID="presenters">
		<rdfs:label>Presenters is a list of Persons</rdfs:label>
		<rdfs:domain rdf:resource="#MultiplePresenterTalk"/>
		<rdfs:domain rdf:resource="#ListOfPersons"/>
	</owl:ObjectProperty>
	<owl:Class rdf:ID="Person">
		<rdfs:comment>There was a previous version that imposed a restriction on Person and thereby
		   created a subclass of contact:Person for the local Person. That was probably rubbish.
		   To make potentially existing data sets o.k., I kept this one here, but it
		   should be deprecated, in fact...</rdfs:comment>
		<owl:equivalentClass rdf:resource="http://www.w3.org/2000/10/swap/pim/contact#Person"/>
	</owl:Class>

	<!-- ============================================================================================== -->
	
	<owl:Class rdf:ID="Event">
		<rdfs:label>An event where a talk is presented, with an extra property that adds the title in English
		(in case the original one is not)</rdfs:label>
		<rdfs:comment>By defining an event to be subClass of ical:Vevent, the talks may be bound to
		    calendaring some day...</rdfs:comment>
		<rdfs:subClassOf rdf:resource="http://www.w3.org/2002/12/cal/ical#Vevent"/>
		<rdfs:subClassOf>
			<owl:Restriction>
				<owl:onProperty rdf:resource="#descriptionEnglish"/>
				<owl:maxCardinality rdf:datatype="http://www.w3.org/2001/XMLSchema#integer">1</owl:maxCardinality>
			</owl:Restriction>
		</rdfs:subClassOf>
		<rdfs:subClassOf>
			<owl:Restriction>
				<owl:onProperty rdf:resource="http://www.w3.org/2001/vcard-rdf/3.0#Locality"/>
				<owl:cardinality rdf:datatype="http://www.w3.org/2001/XMLSchema#integer">1</owl:cardinality>
			</owl:Restriction>
		</rdfs:subClassOf>
		<rdfs:subClassOf>
			<owl:Restriction>
				<owl:onProperty rdf:resource="http://www.w3.org/2001/vcard-rdf/3.0#Country"/>
				<owl:cardinality rdf:datatype="http://www.w3.org/2001/XMLSchema#integer">1</owl:cardinality>
			</owl:Restriction>
		</rdfs:subClassOf>
		<rdfs:subClassOf>
			<owl:Restriction>
				<owl:onProperty rdf:resource="http://www.w3.org/2002/12/cal/ical#description"/>
				<owl:maxCardinality rdf:datatype="http://www.w3.org/2001/XMLSchema#integer">1</owl:maxCardinality>
			</owl:Restriction>
		</rdfs:subClassOf>
		<rdfs:subClassOf>
			<owl:Restriction>
				<owl:onProperty rdf:resource="http://www.w3.org/2002/12/cal/ical#organizer"/>
				<owl:maxCardinality rdf:datatype="http://www.w3.org/2001/XMLSchema#integer">1</owl:maxCardinality>
			</owl:Restriction>
		</rdfs:subClassOf>
		<rdfs:subClassOf>
			<owl:Restriction>
				<owl:onProperty rdf:resource="http://www.w3.org/2002/12/cal/ical#url"/>
				<owl:maxCardinality rdf:datatype="http://www.w3.org/2001/XMLSchema#integer">1</owl:maxCardinality>
			</owl:Restriction>
		</rdfs:subClassOf>
	</owl:Class>
	<owl:DatatypeProperty rdf:ID="descriptionEnglish">
		<rdfs:label>Event Title, strictly in English</rdfs:label>
		<rdfs:domain rdf:resource="#Event"/>
		<rdfs:range rdf:resource="http://www.w3.org/2001/XMLSchema#string"/>
	</owl:DatatypeProperty>
</rdf:RDF>
